Assignment 09

sf/Assignment09_05.v
@@ -5,6 +5,48 @@ Require Export Assignment09_04.
 (** **** Exercise: 2 stars (if_minus_plus)  *)
 (** Prove the following hoare triple using [hoare_if]: *)
 
+Definition basn b : Assertion :=
+  fun st => (beval st b = true).
+
+
+Lemma bexp_eval_true : forall b st,
+  beval st b = true -> (basn b) st.
+Proof.
+  intros b st Hbe.
+  unfold basn.
+  assumption.
+Qed.
+
+Lemma bexp_eval_false : forall b st,
+  beval st b = false -> ~ ((basn b) st).
+Proof.
+  intros b st Hbe contra.
+  unfold basn in contra.
+  rewrite -> contra in Hbe.
+  inversion Hbe.
+Qed.
+
+Theorem hoare_if : forall P Q b c1 c2,
+  {{fun st => P st /\ basn b st}} c1 {{Q}} ->
+  {{fun st => P st /\ ~(basn b st)}} c2 {{Q}} ->
+  {{P}} (IFB b THEN c1 ELSE c2 FI) {{Q}}.
+Proof.
+  intros P Q b c1 c2 HTrue HFalse st st' HE HP.
+  inversion HE; subst.
+  apply (HTrue st st'). 
+  assumption. 
+  split.
+  assumption. 
+  apply bexp_eval_true.
+  assumption.
+  apply (HFalse st st'). 
+  assumption. 
+  split.
+  assumption.
+  apply bexp_eval_false.
+  assumption.
+Qed.
+
 Theorem if_minus_plus :
   {{fun st => True}}
   IFB (BLe (AId X) (AId Y))
@@ -13,7 +55,21 @@ Theorem if_minus_plus :
   FI
   {{fun st => st Y = st X + st Z}}. 
 Proof.
-  exact FILL_IN_HERE.
+  apply hoare_if.
+  eapply hoare_consequence_pre.
+  apply hoare_asgn.
+  unfold basn, assert_implies, assn_sub, update.
+  simpl.
+  intros st [_ H].
+  apply le_plus_minus.
+  apply ble_nat_true in H.
+  assumption.
+  eapply hoare_consequence_pre.
+  apply hoare_asgn.
+  unfold basn, assert_implies, assn_sub, update.
+  simpl.
+  intros st [_ H].
+  reflexivity.
 Qed.
 
 (*-- Check --*)
