sf/Assignment09_01.v
@@ -9,7 +9,14 @@ Theorem assn_sub_ex1:
       X ::= APlus (AId X) (ANum 1)
   {{ fun st => st X <= 5 }}.
 Proof.
-  exact FILL_IN_HERE.
+  unfold hoare_triple.
+  intros.
+  inversion H.
+  subst.
+  inversion H0.
+  simpl.
+  reflexivity.
+  eauto.
 Qed.
 
 (*-- Check --*)
