sf/Assignment09_02.v
@@ -7,7 +7,13 @@ Theorem assn_sub_ex2:
      X ::= ANum 3
   {{ fun st => 0 <= st X /\ st X <= 5 }}.
 Proof.
-  exact FILL_IN_HERE.
+  unfold hoare_triple.
+  intros.
+  inversion H. subst. 
+  inversion H0.
+  split.
+  eapply H1.
+  eapply H2.
 Qed.
 
 (*-- Check --*)
@@ -16,3 +22,5 @@ Check assn_sub_ex2:
      X ::= ANum 3
   {{ fun st => 0 <= st X /\ st X <= 5 }}.
 
+
+ 
