sf/Assignment09_09.v
@@ -45,9 +45,87 @@ Theorem factorial_dec_correct: forall m,
   END
   {{ fun st => st Y = fact m }}.
 Proof.
-  exact FILL_IN_HERE.
+  intros.
+  eapply hoare_consequence_pre with (P' := fun st : state => fact (st X) = fact m).
+  eapply hoare_seq with (Q := fun st : state => (st Y) * fact (st X) = fact m).
+  eapply hoare_consequence_post.
+  eapply hoare_while.
+  eapply hoare_consequence_pre with (P' := fun st : state => (st Y) *(st X) * fact (st X-1) = fact m).
+  eapply hoare_seq with (Q := fun st : state => (st Y) * fact (st X-1) = fact m).
+  eapply hoare_consequence_pre.
+  eapply hoare_asgn.
+  unfold assn_sub.
+  unfold update.
+  unfold assert_implies.
+  intros.
+  assumption.
+  eapply hoare_consequence_pre.
+  eapply hoare_asgn.
+  unfold assn_sub.
+  unfold update.
+  unfold assert_implies.
+  intros.
+  assumption.
+  unfold assert_implies.
+  simpl.
+  intros.
+  induction H.
+  eapply negb_true in H0.
+  eapply beq_nat_false in H0.
+  assert (st X * fact(st X-1) = fact (st X)).
+  Lemma hi : (forall n, n<>0 -> n * fact(n-1) = fact n).
+  Proof.
+    intros.
+    induction n.
+    eapply ex_falso_quodlibet.
+    apply H.
+    reflexivity.
+    simpl.
+    Lemma hi2 : forall n, n-0=n.
+    Proof.
+      induction n.
+      simpl.
+      reflexivity.
+      simpl.
+      reflexivity.
+    Qed.
+    rewrite hi2.
+    reflexivity.
+  Qed.
+  eapply hi.
+  eapply H0.
+  rewrite <- H.
+  rewrite <- H1.
+  Lemma hi3 : forall a b c, a*b*c = a *(b*c).
+  Proof.
+    intros.
+    rewrite <- mult_assoc_reverse.
+    reflexivity.
+  Qed.
+  rewrite <- hi3. 
+  reflexivity.
+  unfold assert_implies.
+  simpl.
+  intros.
+  induction H.
+  eapply negb_false in H0.
+  eapply beq_nat_true in H0.
+  rewrite H0 in H.
+  simpl in H.
+  omega.
+  eapply hoare_consequence_pre.
+  eapply hoare_asgn.
+  unfold assn_sub.
+  unfold update.
+  unfold assert_implies.
+  simpl.
+  intros.
+  omega.
+  unfold assert_implies.
+  intros.
+  rewrite H.
+  reflexivity.
 Qed.
-
 (*-- Check --*)
 Check factorial_dec_correct: forall m,
   {{ fun st => st X = m }} 
