sf/Assignment09_11.v
@@ -11,9 +11,35 @@ Theorem is_wp_example :
   is_wp (fun st => st Y <= 4)
     (X ::= APlus (AId Y) (ANum 1)) (fun st => st X <= 5).
 Proof.
-  exact FILL_IN_HERE.
+  unfold is_wp.
+  split.
+  unfold hoare_triple.
+  intros.
+  inversion H; subst.
+  simpl.
+  unfold update.
+  assert (5 = (4+1)).
+  reflexivity.
+  rewrite H1.
+  apply plus_le_compat_r.
+  apply H0.
+  intros P' ht st P'_holds.
+  unfold hoare_triple in ht.
+  remember (update st X (st Y + 1)) as st'.
+  assert ((X ::= APlus (AId Y) (ANum 1)) / st || st') as E.
+  subst st'.
+  apply E_Ass.
+  reflexivity.
+  apply ht in E.
+  rewrite Heqst' in E.
+  unfold update in E.
+  apply le_pred in E.
+  rewrite plus_comm in E.
+  simpl in E.
+  apply E.
+  assumption.
 Qed.
-
+ 
 (*-- Check --*)
 Check is_wp_example :
   is_wp (fun st => st Y <= 4)
