sf/Assignment09_12.v
@@ -9,7 +9,29 @@ Require Export Assignment09_11.
 Theorem hoare_asgn_weakest : forall Q X a,
   is_wp (Q [X |-> a]) (X ::= a) Q.
 Proof.
-  exact FILL_IN_HERE.
+  unfold is_wp.
+  unfold hoare_triple.
+  unfold assn_sub.
+  unfold update.
+  unfold assert_implies.
+  split.
+    intros.
+    assert (st' = update st X (aeval st a)).
+    apply functional_extensionality.
+    inversion H. subst.
+    reflexivity.
+    rewrite -> H1. 
+    apply H0.
+    intros.
+    remember (update st X (aeval st a)) as st'.
+    assert  ((X ::= a) / st || st').
+    subst.
+    eapply E_Ass.
+    reflexivity.
+    eapply H in H1.
+    subst.
+    eapply H1.
+    eapply H0.
 Qed.
 
 (*-- Check --*)
